{-# OPTIONS --safe #-}
--
module Cubical.Categories.Displayed.Functor.More where

open import Cubical.Foundations.Prelude

open import Cubical.Categories.Category.Base
open import Cubical.Categories.Functor
import      Cubical.Data.Equality as Eq
import      Cubical.Data.Equality.More as Eq

open import Cubical.Categories.Displayed.Base
open import Cubical.Categories.Displayed.Properties
open import Cubical.Categories.Displayed.Functor
open import Cubical.Categories.Displayed.Constructions.Weaken.Base
import      Cubical.Categories.Displayed.Reasoning as HomᴰReasoning

private
  variable
    ℓ ℓB ℓB' ℓC ℓC' ℓCᴰ ℓCᴰ' ℓD ℓD' ℓDᴰ ℓDᴰ' ℓE ℓE' : Level

module _
  {C : Category ℓC ℓC'}{D : Category ℓD ℓD'}
  {Cᴰ : Categoryᴰ C ℓCᴰ ℓCᴰ'}{Dᴰ : Categoryᴰ D ℓDᴰ ℓDᴰ'}
  {F : Functor C D}
  where
  open Functor
  open Functorᴰ
  -- Only use this if H is not refl on ob/hom, otherwise use reindF' below
  reindF : ∀ {G}(H : F ≡ G) → Functorᴰ F Cᴰ Dᴰ → Functorᴰ G Cᴰ Dᴰ
  reindF H = subst (λ F → Functorᴰ F Cᴰ Dᴰ) H

  private
    module C = Category C
    module D = Category D
    module Cᴰ = Categoryᴰ Cᴰ
    module Dᴰ = Categoryᴰ Dᴰ
    module R = HomᴰReasoning Dᴰ

    GF-ob-ty = Eq.singl (F .F-ob)
    GF-hom-ty : GF-ob-ty → Type _
    GF-hom-ty GF-ob = Eq.singlP
      (Eq.ap (λ G-ob → ∀ {x}{y} → C [ x , y ] → D [ G-ob x , G-ob y ])
             (GF-ob .snd))
      (F .F-hom)
  module _ (Fᴰ : Functorᴰ F Cᴰ Dᴰ) where
    open Functor
    reindF'-ob : (GF-ob : GF-ob-ty) → ∀ {x} → Cᴰ.ob[ x ] → Dᴰ.ob[ GF-ob .fst x ]
    reindF'-ob (_ , Eq.refl) = Fᴰ .F-obᴰ

    reindF'-hom : (GF-ob : GF-ob-ty) (GF-hom : GF-hom-ty GF-ob)
                → ∀ {x y}{f : C [ x , y ]}{xᴰ}{yᴰ}
                → Cᴰ [ f ][ xᴰ , yᴰ ]
                → Dᴰ [ GF-hom .fst f
                    ][ reindF'-ob GF-ob xᴰ
                     , reindF'-ob GF-ob yᴰ ]
    reindF'-hom (_ , Eq.refl) (_ , Eq.refl) = Fᴰ .F-homᴰ

    reindF'-id : (GF-ob : GF-ob-ty) (GF-hom : GF-hom-ty GF-ob)
      (GF-id : ∀ {x} → GF-hom .fst (C.id {x}) ≡ D.id)
      → ∀ {x}{xᴰ : Cᴰ.ob[ x ]}
      → reindF'-hom GF-ob GF-hom (Cᴰ.idᴰ {x}{xᴰ}) Dᴰ.≡[ GF-id ] Dᴰ.idᴰ
    reindF'-id (_ , Eq.refl) (_ , Eq.refl) GF-id = R.≡[]-rectify (Fᴰ .F-idᴰ)

    reindF'-seq : (GF-ob : GF-ob-ty) (GF-hom : GF-hom-ty GF-ob)
      (GF-seq : ∀ {x}{y}{z}(f : C [ x , y ])(g : C [ y , z ])
        → GF-hom .fst (f C.⋆ g) ≡ (GF-hom .fst f) D.⋆ GF-hom .fst g)
      → ∀ {x}{y}{z}{f : C [ x , y ]}{g : C [ y , z ]}{xᴰ}{yᴰ}{zᴰ}
      → (fᴰ : Cᴰ [ f ][ xᴰ , yᴰ ]) (gᴰ : Cᴰ [ g ][ yᴰ , zᴰ ]) →
      reindF'-hom GF-ob GF-hom
      (fᴰ Cᴰ.⋆ᴰ gᴰ) Dᴰ.≡[ GF-seq f g ]
      reindF'-hom GF-ob GF-hom fᴰ Dᴰ.⋆ᴰ reindF'-hom GF-ob GF-hom gᴰ
    reindF'-seq (_ , Eq.refl) (_ , Eq.refl) GF-seq fᴰ gᴰ =
      R.≡[]-rectify (Fᴰ .F-seqᴰ fᴰ gᴰ)

  open Functor
  -- This is preferable to reindF if the equalities are Refl.
  reindF' : (G : Functor C D)
            (GF-ob≡FF-ob : F .F-ob Eq.≡ G .F-ob)
            (GF-hom≡FF-hom :
              Eq.HEq (Eq.ap (λ F-ob₁ → ∀ {x} {y}
                         → C [ x , y ] → D [ F-ob₁ x , F-ob₁ y ])
                         GF-ob≡FF-ob)
                (F .F-hom)
                (G .F-hom))
          → Functorᴰ F Cᴰ Dᴰ
          → Functorᴰ G Cᴰ Dᴰ
  reindF' G GF-ob≡FF-ob GF-hom≡FF-hom Fᴰ = record
    { F-obᴰ  = reindF'-ob Fᴰ GF-ob
    ; F-homᴰ = reindF'-hom Fᴰ GF-ob GF-hom
    ; F-idᴰ  = reindF'-id Fᴰ GF-ob GF-hom (G .F-id)
    ; F-seqᴰ = reindF'-seq Fᴰ GF-ob GF-hom (G .F-seq)
    } where
      GF-ob : GF-ob-ty
      GF-ob = _ , GF-ob≡FF-ob

      GF-hom : GF-hom-ty GF-ob
      GF-hom = _ , GF-hom≡FF-hom
